Some improvements and cleanup regarding global initializers

progs/global.c
@@ -1,6 +1,23 @@
+struct foo {int x; char a[2];};
+
+struct foo *p;
+
+struct foo a;
+
+struct foo b = {5,{6,7}};
+
+struct foo c = {5};
+
+struct foo d = {5,6};
+
+struct foo e[3];
+
+struct foo f[3] = {{1,{2,3}},{4,{5,6}},{7,"x"}};
+
 int g = 7;
 
-int f(void) {
+
+int h(void) {
   int x;
   x = g;
   return x;
@@ -8,6 +25,7 @@ int f(void) {
 
 int main(void) {
   int y;
-  y = f();
+  y = h();
   return y;
 }
+
