progs/verif_global.v
@@ -3,8 +3,8 @@ Require Import VST.progs.global.
 Instance CompSpecs : compspecs. make_compspecs prog. Defined.
 Definition Vprog : varspecs.  mk_varspecs prog. Defined.
 
-Definition f_spec :=
- DECLARE _f
+Definition h_spec :=
+ DECLARE _h
   WITH gv: globals
   PRE [  ]
           PROP  ()
@@ -21,9 +21,9 @@ Definition main_spec :=
   POST [ tint ] main_post prog [] gv.
 
 Definition Gprog : funspecs :=
-        ltac:(with_library prog [f_spec; main_spec]).
+        ltac:(with_library prog [h_spec; main_spec]).
 
-Lemma body_f: semax_body Vprog Gprog f_f f_spec.
+Lemma body_h: semax_body Vprog Gprog f_h h_spec.
 Proof.
 start_function.
 forward.  (* x = g; *)
