veric/mapsto_memory_block.v
@@ -386,8 +386,9 @@ Qed.
 
 Definition mapsto_zeros (n: Z) (sh: share) (a: val) : mpred :=
  match a with
-  | Vptr b z => address_mapsto_zeros sh (nat_of_Z n)
-                          (b, Ptrofs.unsigned z)
+  | Vptr b z => 
+    !! (0 <= Ptrofs.unsigned z  /\ n + Ptrofs.unsigned z < Ptrofs.modulus)%Z &&
+    address_mapsto_zeros sh (nat_of_Z n) (b, Ptrofs.unsigned z)
   | _ => TT
   end.
 
@@ -406,7 +407,7 @@ Definition memory_block'_alt (sh: share) (n: nat) (b: block) (ofs: Z) : mpred :=
 Lemma memory_block'_eq:
  forall sh n b i,
   0 <= i ->
-  Z_of_nat n + i <= Ptrofs.modulus ->
+  Z_of_nat n + i < Ptrofs.modulus ->
   memory_block' sh n b i = memory_block'_alt sh n b i.
 Proof.
   intros.
@@ -772,6 +773,18 @@ Proof.
     auto.
 Qed.
 
+Lemma Nat2Z_add_lt: forall n i, Ptrofs.unsigned i + n < Ptrofs.modulus ->
+  Z.of_nat (nat_of_Z n) + Ptrofs.unsigned i < Ptrofs.modulus.
+Proof.
+  intros.
+  destruct (zle 0 n).
+  + rewrite Coqlib.nat_of_Z_eq by omega. omega.
+  + rewrite nat_of_Z_neg by omega.
+    pose proof Ptrofs.unsigned_range i.
+    simpl.
+    omega.
+Qed.
+
 Lemma Nat2Z_add_le: forall n i, Ptrofs.unsigned i + n <= Ptrofs.modulus ->
   Z.of_nat (nat_of_Z n) + Ptrofs.unsigned i <= Ptrofs.modulus.
 Proof.
@@ -794,9 +807,9 @@ Proof.
   rewrite sepcon_andp_prop1.
   rewrite sepcon_andp_prop2.
   apply normalize.derives_extract_prop; intros.
-  apply normalize.derives_extract_prop; intros.
-  rewrite memory_block'_eq; [| pose proof Ptrofs.unsigned_range i; omega | apply Nat2Z_add_le; omega].
-  rewrite memory_block'_eq; [| pose proof Ptrofs.unsigned_range i0; omega | apply Nat2Z_add_le; omega].
+  apply normalize.derives_extract_prop; intros. 
+  rewrite memory_block'_eq; [| pose proof Ptrofs.unsigned_range i; omega | apply Nat2Z_add_lt; omega].
+  rewrite memory_block'_eq; [| pose proof Ptrofs.unsigned_range i0; omega | apply Nat2Z_add_lt; omega].
   unfold memory_block'_alt.
   if_tac.
   + clear H2.
@@ -895,25 +908,31 @@ Proof.
 Qed.
 
 Lemma mapsto_zeros_memory_block: forall sh n b ofs,
-  n < Ptrofs.modulus ->
+(*  n < Ptrofs.modulus ->
   Ptrofs.unsigned ofs+n < Ptrofs.modulus ->
-  readable_share sh ->
+*)  readable_share sh ->
   mapsto_zeros n sh (Vptr b ofs) |--
   memory_block sh n (Vptr b ofs).
 Proof.
   unfold mapsto_zeros.
-  intros.
-  rename H0 into H'. rename H1 into RS.
+  intros. rename H into RS. pose proof I.
+(*  rename H0 into H'. rename H1 into RS. *)
   unfold memory_block.
   destruct (zlt n 0).   {
-     rewrite nat_of_Z_neg by omega. simpl. rewrite prop_true_andp by auto. auto.
+     rewrite nat_of_Z_neg by omega. simpl.
+     apply andp_derives; auto.
+     intros ? ?. simpl in *. destruct H0.
+     omega. 
   }
- assert (0 <= n < Ptrofs.modulus) by omega. clear H g; rename H0 into H.
-  repeat rewrite Int.unsigned_repr by omega.
-  apply andp_right.
-  + intros ? _; auto.
-  + rewrite <- (Z2Nat.id n) in H' by omega.
-    rewrite <- (Z2Nat.id n) in H by omega.
+ apply prop_andp_left; intros [? ?].
+ rewrite prop_true_andp by omega.
+ assert (n <= Ptrofs.modulus) by omega. clear H H0. rename H1 into H'.
+ assert (0 <= n <= Ptrofs.modulus) by omega. clear H2 g.
+(*  repeat rewrite Int.unsigned_repr by omega. 
+  apply andp_right.  
+  + intros ? _; auto. 
+  + *)
+    rewrite <- (Z2Nat.id n) in H', H by omega.
     change nat_of_Z with Z.to_nat.
     forget (Z.to_nat n) as n'.
     clear n.
@@ -954,7 +973,7 @@ Qed.
 Lemma memory_block'_split:
   forall sh b ofs i j,
    0 <= i <= j ->
-    j <= j+ofs <= Ptrofs.modulus ->
+    j <= j+ofs < Ptrofs.modulus ->
    memory_block' sh (nat_of_Z j) b ofs =
       memory_block' sh (nat_of_Z i) b ofs * memory_block' sh (nat_of_Z (j-i)) b (ofs+i).
 Proof.
